disk-betree/DiskBetreeRefinement.dfy
@@ -1,91 +1,61 @@
 include "DiskBetree.dfy"
 include "MapSpec.dfy"
-  
+include "DiskBetreeInv.dfy"
+
 abstract module DiskBetreeRefinement {
-  import opened DiskBetree
+  import opened DiskBetreeInv
 
-  /// Invariants
-  
-  predicate KeyHasSatisfyingLookup<Value(!new)>(k: Constants, s: Variables, key: Key)
-  {
-    exists lookup, value :: IsSatisfyingLookup(k, s, key, value, lookup)
-  }
-
-  predicate Inv(k: Constants, s: Variables)
-  {
-    forall key | MS.InDomain(key) :: KeyHasSatisfyingLookup(k, s, key)
-  }
-
-  lemma InitImpliesInv(k: Constants, s: Variables)
-    requires Init(k, s)
-    ensures Inv(k, s)
-  {
-    assert forall key :: MS.InDomain(key) ==> IsSatisfyingLookup(k, s, key, MS.EmptyValue(), [Layer(BC.Root(k.bcc), EmptyNode(), [Insertion(MS.EmptyValue())])]);
-  }
-
-  lemma NextStepPreservesInvariant(k: Constants, s: Variables, s': Variables, step: Step)
-    requires Inv(k, s)
-    requires NextStep(k, s, s', step)
-    ensures Inv(k, s')
+  type Key = DB.Key
+  type Lookup<Value> = DB.Lookup<Value>
     
-  lemma NextPreservesInvariant(k: Constants, s: Variables, s': Variables)
-    requires Inv(k, s)
-    requires Next(k, s, s')
-    ensures Inv(k, s')
-  {
-    var step :| NextStep(k, s, s', step);
-    NextStepPreservesInvariant(k, s, s', step);
-  }
-    
-  // Refinement proof
-
   datatype Pair<S,T> = Pair(first: S, second: T)
   
-  function GetLookup<Value>(k: Constants, s: Variables, key: Key) : Pair<Lookup, Value>
-    requires KeyHasSatisfyingLookup(k, s, key);
+  function GetLookup<Value>(k: DB.Constants, s: DB.Variables, key: Key) : Pair<Lookup, Value>
+    requires DB.KeyHasSatisfyingLookup(k, s, key);
   {
-    var lookup, value :| IsSatisfyingLookup(k, s, key, value, lookup);
+    var lookup, value :| DB.IsSatisfyingLookup(k, s, key, value, lookup);
     Pair(lookup, value)
   }
 
-  function GetValue<Value>(k: Constants, s: Variables, key: Key) : Value
-    requires KeyHasSatisfyingLookup(k, s, key);
+  function GetValue<Value>(k: DB.Constants, s: DB.Variables, key: Key) : Value
+    requires DB.KeyHasSatisfyingLookup(k, s, key);
   {
     GetLookup(k, s, key).second
   }
   
-  function Ik(k: Constants) : MS.Constants {
-    MS.Constants()
+  function Ik(k: DB.Constants) : DB.MS.Constants {
+    DB.MS.Constants()
   }
   
-  function I(k: Constants, s: Variables) : MS.Variables
+  function I(k: DB.Constants, s: DB.Variables) : DB.MS.Variables
     requires Inv(k, s)
   {
-    MS.Variables(imap key | MS.InDomain(key) :: GetValue(k, s, key))
+    DB.MS.Variables(imap key | DB.MS.InDomain(key) :: GetValue(k, s, key))
   }
 
-  lemma BetreeRefinesMapInit(k: Constants, s: Variables)
-    requires Init(k, s)
+  lemma BetreeRefinesMapInit(k: DB.Constants, s: DB.Variables)
+    requires DB.Init(k, s)
     ensures Inv(k, s)
-    ensures MS.Init(Ik(k), I(k, s))
+    ensures DB.MS.Init(Ik(k), I(k, s))
   {
     InitImpliesInv(k, s);
   }
 
-  lemma BetreeRefinesMapNextStep(k: Constants, s: Variables, s':Variables, step: Step)
+  lemma BetreeRefinesMapNextStep(k: DB.Constants, s: DB.Variables, s':DB.Variables, step: DB.Step)
     requires Inv(k, s)
-    requires NextStep(k, s, s', step)
-    ensures MS.Next(Ik(k), I(k, s), I(k, s'))
-    
-    
-  lemma BetreeRefinesMapNext(k: Constants, s: Variables, s':Variables)
-    requires Inv(k, s)
-    requires Next(k, s, s')
+    requires DB.NextStep(k, s, s', step)
     ensures Inv(k, s')
-    ensures MS.Next(Ik(k), I(k, s), I(k, s'))
+    ensures DB.MS.Next(Ik(k), I(k, s), I(k, s'))
+    
+    
+  lemma BetreeRefinesMapNext(k: DB.Constants, s: DB.Variables, s':DB.Variables)
+    requires Inv(k, s)
+    requires DB.Next(k, s, s')
+    ensures Inv(k, s')
+    ensures DB.MS.Next(Ik(k), I(k, s), I(k, s'))
   {
     NextPreservesInvariant(k, s, s');
-    var step :| NextStep(k, s, s', step);
+    var step :| DB.NextStep(k, s, s', step);
     BetreeRefinesMapNextStep(k, s, s', step);
   }
 }
