disk-betree/DiskBetreeInv.dfy
@@ -1,0 +1,36 @@
+include "MapSpec.dfy"
+include "DiskBetree.dfy"
+  
+abstract module DiskBetreeInv {
+  import opened DB : DiskBetree
+
+  /// Invariants
+  
+  predicate Inv(k: Constants, s: Variables)
+  {
+    forall key | MS.InDomain(key) :: KeyHasSatisfyingLookup(k, s, key)
+  }
+
+  lemma InitImpliesInv(k: Constants, s: Variables)
+    requires Init(k, s)
+    ensures Inv(k, s)
+  {
+    assert forall key :: MS.InDomain(key) ==> IsSatisfyingLookup(k, s, key, MS.EmptyValue(), [Layer(BC.Root(k.bcc), EmptyNode(), [Insertion(MS.EmptyValue())])]);
+  }
+
+  lemma NextStepPreservesInvariant(k: Constants, s: Variables, s': Variables, step: Step)
+    requires Inv(k, s)
+    requires NextStep(k, s, s', step)
+    ensures Inv(k, s')
+    
+  lemma NextPreservesInvariant(k: Constants, s: Variables, s': Variables)
+    requires Inv(k, s)
+    requires Next(k, s, s')
+    ensures Inv(k, s')
+  {
+    var step :| NextStep(k, s, s', step);
+    NextStepPreservesInvariant(k, s, s', step);
+  }
+    
+
+}
